{-# OPTIONS --prop #-}

module sign-analysis where


open import Data.Unit using (âŠ¤; tt)
open import Data.Empty using (âŠ¥)
open import Data.Integer using (â„¤; +_; -[1+_])
  renaming (_+_ to _+â„¤_; _*_ to _*â„¤_)
open import Data.Nat using (zero; suc)
open import Data.Bool using (false; true; if_then_else_) 
  renaming (_â‰¤_ to _â‰¤ğ”¹_; Bool to ğ”¹; _âˆ§_ to _âˆ§ğ”¹_; _âˆ¨_ to _âˆ¨ğ”¹_)
open import Signs
open import Relation.Binary.PropositionalEquality
  using (_â‰¡_; refl)
open import Data.Product using (âˆƒ-syntax; âˆƒ; _,_)


Î± : â„¤ -> Sgns
Î± (+_ zero) = sg z
Î± (+_ (suc n)) = sg +
Î± (-[1+_] n) = sg -


-- +-sgns : Sgns -> Sgns -> 

data Expr : Set where
  I   : â„¤ -> Expr
  _+_ : Expr -> Expr -> Expr
  _*_ : Expr -> Expr -> Expr


eval : Expr -> â„¤
eval (I x) = x
eval (c1 + c2) = eval c1 +â„¤ eval c2
eval (c1 * c2) = eval c1 *â„¤ eval c2

eval^ : Expr -> Sgns
eval^ (I x) = Î± x
eval^ (e1 + e2) = (eval^ e1) +^ (eval^ e2)
eval^ (e1 * e2) = (eval^ e1) *^ (eval^ e2)

pos : â„¤ -> Set
pos v = Î± v â‰¡ sg +

pos-lem1 : (n : â„¤) -> pos n -> âˆƒ[ m ] (+_ (suc m) â‰¡ n)
pos-lem1 (+_ (suc n)) p = n , refl


pos+pos : (v1 v2 : â„¤) -> (pos v1) -> (pos v2) -> pos (v1 +â„¤ v2)
pos+pos n m p1 p2 with pos-lem1 n p1 | pos-lem1 m p2 
... | n+ , refl | m+ , refl = refl

pos+z : (v1 v2 : â„¤) -> (pos v1) -> (pos v2) -> pos (v1 +â„¤ v2)
pos+z n m p1 p2 with pos-lem1 n p1 | pos-lem1 m p2 
... | n+ , refl | m+ , refl = refl


Î±+-homo : âˆ€ (v1 v2 : â„¤) -> ((Î± (v1 +â„¤ v2)) â‰¤ (Î± v1 +^ Î± v2))
Î±+-homo (+_ zero) (+_ zero) = tt
Î±+-homo (+_ (suc n)) (+_ zero) = tt
Î±+-homo (+_ zero) (+_ (suc m)) = tt
Î±+-homo (+_ (suc n)) (+_ (suc m)) = tt
Î±+-homo (+_ zero) (-[1+_] nâ‚) = tt
Î±+-homo (+_ (suc n)) (-[1+_] nâ‚) = ge-âŠ¤
Î±+-homo (-[1+_] n) (+_ zero) = tt
Î±+-homo (-[1+_] n) (+_ (suc nâ‚)) = ge-âŠ¤
Î±+-homo (-[1+_] n) (-[1+_] nâ‚) = tt



soundness : (e : Expr) -> (Î± (eval e) â‰¤ eval^ e)
soundness (I x) = refl-â‰¤
soundness (e1 + e2) with soundness e1 | soundness e2
... |  pf1 | pf2 = trans (Î±+-homo (eval e1) (eval e2)) {!!}
soundness (e1 * e2) = {!!}







